Work on relocation proof.  Changed statement after consulting with Stephen following problems with last statement.  New statement is slightly easier to work with and progress is being made!!

prf/ELF_Relocation_Proof.thy
@@ -39,30 +39,25 @@ fun run_program :: "instruction list \<Rightarrow> X64_state \<Rightarrow> X64_s
      (let (_, \<sigma>') = Run x \<sigma> in
        run_program xs \<sigma>')"
 
-fun X64_memory_of_elf64_interpreted_segments :: "elf64_interpreted_segment list \<Rightarrow> 64 word \<Rightarrow> 8 word" where
-  "X64_memory_of_elf64_interpreted_segments segs addr =
-     (case (filter (\<lambda>x. elf64_segment_base x \<le> unat addr \<and> elf64_segment_base x + elf64_segment_size x \<le> unat addr) segs) of
-       [] \<Rightarrow> undefined
-     | [x] \<Rightarrow>
-       if elf64_segment_type x = elf_pt_load then
-         let off = unat addr - elf64_segment_base x in
-         (case elf64_segment_body x of
-            Sequence s \<Rightarrow>
-              List.nth s (elf64_segment_base x - unat addr))
-       else
-         undefined
-     | x#xs \<Rightarrow> undefined)"
+fun X64_memory_of_memory_image :: "memory_image \<Rightarrow> (nat \<Rightarrow> 8 word)" where
+  "X64_memory_of_memory_image i addr =
+     (let keys = Map.dom i in
+      let rels = { s. \<forall>k \<in> keys. Some s = i k \<and> addr \<ge> the (startpos s) \<and> addr \<le> the (startpos s) + the (length1 s) } in
+      let arb  = Set.the_elem rels in
+      let reba = addr - the (startpos arb) in
+      let byte = List.nth (contents arb) reba in
+        the byte)"
 
-definition load_image :: "elf64_interpreted_segment list \<Rightarrow> nat \<Rightarrow> X64_state" where
-  "load_image segs entry_point \<equiv>
+definition load_image :: "memory_image \<Rightarrow> nat \<Rightarrow> X64_state" where
+  "load_image i entry_point \<equiv>
      \<lparr> EFLAGS = \<lambda>x. None (* XXX: or False? *)
-     , MEM = X64_memory_of_elf64_interpreted_segments segs
+     , MEM = \<lambda>a. X64_memory_of_memory_image i (unat a)
      , REG = \<lambda>x. (0 :: 64 word)
      , RIP = of_nat entry_point
      , exception = NoException
      \<rparr>"
 
-fun execute_two_steps :: "X64_state \<Rightarrow> X64_state" where
+definition execute_two_steps :: "X64_state \<Rightarrow> X64_state" where
   "execute_two_steps \<sigma> =
      (let (fetched, \<sigma>') = x64_fetch \<sigma> in
       let decoded = x64_decode fetched in
@@ -78,12 +73,12 @@ fun execute_two_steps :: "X64_state \<Rightarrow> X64_state" where
               | _ \<Rightarrow> undefined))
        | _ \<Rightarrow> undefined))"
 
-definition initial_state :: "X64_state" where
-  "initial_state \<equiv>
+definition initial_state :: "nat \<Rightarrow> X64_state" where
+  "initial_state entry \<equiv>
     \<lparr> EFLAGS = \<lambda>x. None
     , MEM = \<lambda>addr. 0
     , REG = \<lambda>x. 0
-    , RIP = 0
+    , RIP = of_nat entry
     , exception = NoException
     \<rparr>"
 
@@ -99,110 +94,143 @@ by (cases z, auto)
  *   run_program fixed_program empty_state \<simeq> execute_two_steps \<sigma>0
  *)
 
-lemma silly_map_lemma1:
-  shows "List.concat (map encode [mov_constant_to_mem 5 0, mov_constant_from_mem 0]) =
-    [72, 199, 4, 37, 0, 0, 0, 0, 5, 0, 0, 0, 72, 139, 4, 37, 0, 0, 0, 0]"
+definition relocation_test :: "nat \<Rightarrow> bool error" where
+  "relocation_test entry \<equiv>
+     (let i = elements relocation_image in
+      let rstate = load_image i entry in
+      let final_fixed_state = run_program fixed_program (initial_state entry) in
+      let final_relocatable_state = execute_two_steps rstate in
+        Success (REG final_fixed_state = REG final_relocatable_state))"
+
+lemma swap_pairs_lemma:
+  shows "swap_pairs {(Some (''.text'', 1, 4), SymbolRef ref_and_reloc_rec0), (Some (''.data'', 0, 8), SymbolDef def_rec0)} =
+      {(SymbolRef ref_and_reloc_rec0, Some (''.text'', 1, 4)), (SymbolDef def_rec0, Some (''.data'', 0, 8))}"
+  apply(simp add: swap_pairs_def)
+  apply auto
+done
+
+(* XXX: ugly, but necessary to control the simplifier below *)
+lemma for_loop_19_unroll:
+  fixes act :: "nat \<Rightarrow> 'a \<Rightarrow> (unit \<times> 'a)"
+  shows "for_loop ((19::nat), 0, act) = (\<lambda>u. case act 19 u of
+     (u, ua) \<Rightarrow> case act 18 ua of
+                (u, ua) \<Rightarrow> case act 17 ua of
+                           (u, ua) \<Rightarrow> case act 16 ua of
+                                      (u, ua) \<Rightarrow> case act 15 ua of
+                                                 (u, ua) \<Rightarrow> case act 14 ua of
+                                                            (u, ua) \<Rightarrow> case act 13 ua of
+                                                                       (u, ua) \<Rightarrow> case act 12 ua of
+                                                                                  (u, ua) \<Rightarrow> case act 11 ua of
+                                                                                             (u, ua) \<Rightarrow> case act 10 ua of
+     (u, ua) \<Rightarrow> case act 9 ua of
+                (u, ua) \<Rightarrow> case act 8 ua of
+                           (u, ua) \<Rightarrow> case act 7 ua of
+                                      (u, ua) \<Rightarrow> case act 6 ua of
+                                                 (u, ua) \<Rightarrow> case act 5 ua of
+                                                            (u, ua) \<Rightarrow> case act 4 ua of (u, ua) \<Rightarrow> case act 3 ua of (u, ua) \<Rightarrow> case act 2 ua of (u, ua) \<Rightarrow> case act 1 ua of (u, x) \<Rightarrow> act 0 x)"
+  by simp
+ 
+lemma dom_lemma:
+  shows "{a. [''.text'' \<mapsto>
+                      \<lparr>startpos = Some 4194304, length1 = Some 16,
+                         contents = map Some (e_rm_imm (Z64, Zm (None, ZnoBase, 0), 5, 0, 198)) @ map Some (e_rm_reg (Z64, Zm (None, ZnoBase, 0), word_of_int (int (Zreg_to_nat RAX)), [], 138))\<rparr>,
+                      ''.data'' \<mapsto> \<lparr>startpos = Some 4194320, length1 = Some 8, contents = map Some (replicate 8 (of_nat 42))\<rparr>]
+                      a \<noteq>
+                     None} = { ''.text'', ''.data''}"
+  by auto
+
+lemma rels_lemma:
+  shows "{s. \<forall>k\<in>{''.text'', ''.data''}.
+                        Some s = [''.text'' \<mapsto>
+                                  \<lparr>startpos = Some 4194304, length1 = Some 16,
+                                     contents = map Some (e_rm_imm (Z64, Zm (None, ZnoBase, 0), 5, 0, 198)) @
+                                                map Some (e_rm_reg (Z64, Zm (None, ZnoBase, 0), word_of_int (int (Zreg_to_nat RAX)), [], 138))\<rparr>,
+                                  ''.data'' \<mapsto> \<lparr>startpos = Some 4194320, length1 = Some 8, contents = map Some (replicate 8 (of_nat 42))\<rparr>]
+                                  k \<and>
+                        the (startpos s) \<le> unat (of_nat 4194304 + word_of_int (int 0)) \<and> unat (of_nat 4194304 + word_of_int (int 0)) \<le> the (startpos s) + the (length1 s)} =
+                               { \<lparr>startpos = Some 4194304, length1 = Some 16,
+                                            contents = map Some (e_rm_imm (Z64, Zm (None, ZnoBase, 0), 5, 0, 198)) @
+                                                       map Some (e_rm_reg (Z64, Zm (None, ZnoBase, 0), word_of_int (int (Zreg_to_nat RAX)), [], 138))\<rparr> }"
 sorry
 
-lemma silly_map_lemma2:
-  shows "map Some [72, 199, 4, 37, 0, 0, 0, 0, 5, 0, 0, 0, 72, 139, 4, 37, 0, 0, 0, 0] =
-    [Some 72, Some 199, Some 4, Some 37, Some 0, Some 0, Some 0, Some 0, Some 5, Some 0, Some 0,
-       Some 0, Some 72, Some 139, Some 4, Some 37, Some 0, Some 0, Some 0, Some 0]"
-by auto
+lemma the_elem_lemma:
+  shows "the_elem {\<lparr>startpos = Some 4194304, length1 = Some 16,
+                             contents = map Some (e_rm_imm (Z64, Zm (None, ZnoBase, 0), 5, 0, 198)) @
+                                        map Some (e_rm_reg (Z64, Zm (None, ZnoBase, 0), word_of_int (int (Zreg_to_nat RAX)), [], 138))\<rparr>} =
+                                        \<lparr>startpos = Some 4194304, length1 = Some 16,
+                             contents = map Some (e_rm_imm (Z64, Zm (None, ZnoBase, 0), 5, 0, 198)) @
+                                        map Some (e_rm_reg (Z64, Zm (None, ZnoBase, 0), word_of_int (int (Zreg_to_nat RAX)), [], 138))\<rparr>"
+  by auto
 
-lemma silly_rev_lemma1:
-  shows "rev [(''.text'', \<lparr>startpos = Some 4194304, length1 = Some 16,
-           contents = [Some 72, Some 199, Some 4, Some 37, Some 0, Some 0, Some 0, Some 0, Some 5, Some 0, Some 0, Some 0, Some 72, Some 139,
-             Some 4, Some 37, Some 0, Some 0, Some 0, Some 0]\<rparr>),
-           (''.data'', \<lparr>startpos = Some 4194320, length1 = Some 8, contents = map Some (replicate 8 (of_nat 42))\<rparr>)] =
-  [(''.data'', \<lparr>startpos = Some 4194320, length1 = Some 8, contents = map Some (replicate 8 (of_nat 42))\<rparr>),
-   (''.text'', \<lparr>startpos = Some 4194304, length1 = Some 16,
-           contents = [Some 72, Some 199, Some 4, Some 37, Some 0, Some 0, Some 0, Some 0, Some 5, Some 0, Some 0, Some 0, Some 72, Some 139,
-             Some 4, Some 37, Some 0, Some 0, Some 0, Some 0]\<rparr>)]"
-by simp
+lemma word_calc_lemma:
+  shows "unat (of_nat 4194304 + word_of_int (int 0)) = 4194304"
+sorry
 
-lemma silly_rev_lemma2:
-  shows "rev [(''test'', [(0, (0, ref_rec0, ref_linkable_item), Some (0, def_rec0, ref_linkable_item))])]
-    = [(''test'', [(0, (0, ref_rec0, ref_linkable_item), Some (0, def_rec0, ref_linkable_item))])]"
-by auto
+lemma the_startpos_lemma:
+  shows "the (startpos \<lparr>startpos = Some 4194304, length1 = Some 16,
+                                  contents = map Some (e_rm_imm (Z64, Zm (None, ZnoBase, 0), 5, 0, 198)) @
+                                             map Some (e_rm_reg (Z64, Zm (None, ZnoBase, 0), word_of_int (int (Zreg_to_nat RAX)), [], 138))\<rparr>) = 4194304"
+  by auto
 
-lemma silly_map_of_lemma1:
-  shows "map_of [(''.data'', \<lparr>startpos = Some 4194320, length1 = Some 8, contents = map Some (replicate 8 (of_nat 42))\<rparr>),
-                                                          (''.text'',
-                                                           \<lparr>startpos = Some 4194304, length1 = Some 16,
-                                                              contents = [Some 72, Some 199, Some 4, Some 37, Some 0, Some 0, Some 0, Some 0, Some 5, Some 0, Some 0, Some 0, Some 72, Some 139,
-                                                                          Some 4, Some 37, Some 0, Some 0, Some 0, Some 0]\<rparr>)]
-    = (\<lambda>x. if x = ''.data'' then 
-        Some \<lparr>startpos = Some 4194320, length1 = Some 8, contents = map Some (replicate 8 (of_nat 42))\<rparr>
-     else if x = ''.text'' then
-       Some \<lparr>startpos = Some 4194304, length1 = Some 16,
-                                                              contents = [Some 72, Some 199, Some 4, Some 37, Some 0, Some 0, Some 0, Some 0, Some 5, Some 0, Some 0, Some 0, Some 72, Some 139,
-                                                                          Some 4, Some 37, Some 0, Some 0, Some 0, Some 0]\<rparr>
-     else
-       None)"
-by auto
-
-lemma silly_map_of_lemma2:
-  shows "map_of [(''test'', [(0, (0, ref_rec0, ref_linkable_item), Some (0, def_rec0, ref_linkable_item))])] =
-    (\<lambda>x. if x = ''test'' then Some [(0, (0, ref_rec0, ref_linkable_item), Some (0, def_rec0, ref_linkable_item))] else None)"
-by auto
-
-lemma silly_let_lemma:
-  shows "let initial_img =
-                                      \<lparr>elements = \<lambda>x. if x = ''.data'' then Some \<lparr>startpos = Some 4194320, length1 = Some 8, contents = map Some (replicate 8 (of_nat 42))\<rparr>
-                                                      else if x = ''.text''
-                                                           then Some \<lparr>startpos = Some 4194304, length1 = Some 16,
-                                                                        contents = [Some 72, Some 199, Some 4, Some 37, Some 0, Some 0, Some 0, Some 0, Some 5, Some 0, Some 0, Some 0, Some 72,
-                                                                                    Some 139, Some 4, Some 37, Some 0, Some 0, Some 0, Some 0]\<rparr>
-                                                           else None,
-                                         by_range = set meta0, by_tag = by_tag_from_by_range (set meta0)\<rparr>;
-                                    ref_input_item = (''test.o'', Reloc (Sequence []), File (Filename ''blah'', null_input_file_options), [InCommandLine 0]);
-                                    ref_linkable_item = (RelocELF initial_img, ref_input_item, null_input_options);
-                                    bindings_by_name = \<lambda>x. if x = ''test'' then Some [(0, (0, ref_rec0, ref_linkable_item), Some (0, def_rec0, ref_linkable_item))] else None
-                                in relocate_output_image sysv_amd64_std_abi bindings_by_name initial_img
-  = relocate_output_image sysv_amd64_std_abi (\<lambda>x. if x = ''test'' then Some [(0, (0, ref_rec0, (RelocELF initial_img, (''test.o'', Reloc (Sequence []), File (Filename ''blah'', null_input_file_options), [InCommandLine 0]), null_input_options)), Some (0, def_rec0, (RelocELF initial_img, (''test.o'', Reloc (Sequence []), File (Filename ''blah'', null_input_file_options), [InCommandLine 0]), null_input_options)))] else None) \<lparr>elements = \<lambda>x. if x = ''.data'' then Some \<lparr>startpos = Some 4194320, length1 = Some 8, contents = map Some (replicate 8 (of_nat 42))\<rparr>
-                                                      else if x = ''.text''
-                                                           then Some \<lparr>startpos = Some 4194304, length1 = Some 16,
-                                                                        contents = [Some 72, Some 199, Some 4, Some 37, Some 0, Some 0, Some 0, Some 0, Some 5, Some 0, Some 0, Some 0, Some 72,
-                                                                                    Some 139, Some 4, Some 37, Some 0, Some 0, Some 0, Some 0]\<rparr>
-                                                           else None,
-                                         by_range = set meta0, by_tag = by_tag_from_by_range (set meta0)\<rparr>"
-by auto
-
-definition relocation_test :: "bool error" where
-  "relocation_test \<equiv>
-     (let ef = elf64_file_of_elf_memory_image sysv_amd64_std_abi id ''at_least_some_relocations_relocate.out'' relocation_image in
-      get_elf64_executable_image ef >>= (\<lambda>(segs_and_provenance, entry, machine).
-        if \<not> (machine = elf_ma_x86_64) then
-          Fail ''machine type incorrect''
-        else
-          let rstate = load_image (List.map fst segs_and_provenance) entry in
-          let final_fixed_state = run_program fixed_program initial_state in
-          let final_relocatable_state = execute_two_steps rstate in
-            return (REG final_fixed_state = REG final_relocatable_state)))"
+lemma x64_fetch_lemma:
+  shows "x64_fetch \<lparr>EFLAGS = Map.empty,
+                       MEM = \<lambda>a\<Colon>64 word. X64_memory_of_memory_image
+                                          [''.text'' \<mapsto>
+                                           \<lparr>startpos = Some (4194304\<Colon>nat), length1 = Some (16\<Colon>nat),
+                                              contents = map Some (e_rm_imm (Z64, Zm (None, ZnoBase, 0\<Colon>64 word), 5\<Colon>64 word, 0\<Colon>4 word, 198\<Colon>8 word)) @
+                                                         map Some (e_rm_reg (Z64, Zm (None, ZnoBase, 0\<Colon>64 word), word_of_int (int (Zreg_to_nat RAX)), [], 138\<Colon>8 word))\<rparr>,
+                                           ''.data'' \<mapsto> \<lparr>startpos = Some (4194320\<Colon>nat), length1 = Some (8\<Colon>nat), contents = map Some (replicate (8\<Colon>nat) (of_nat (42\<Colon>nat)))\<rparr>]
+                                          (unat a),
+                       REG = \<lambda>x\<Colon>Zreg. 0\<Colon>64 word, RIP = of_nat (4194304\<Colon>nat), exception = NoException\<rparr> = xxx"
+  apply(simp only: x64_fetch.simps)
+  apply(simp only: Let_def)
+  apply(simp only: for_loop_19_unroll)
+  apply(simp only: split fst_def snd_def)
+  apply(simp only: X64_state.simps)
+  apply(simp only: X64_memory_of_memory_image.simps)
+  apply(simp only: dom_def)
+  apply(simp only: dom_lemma)
+  apply(subst Let_def)
+  apply(simp only: let_weak_cong[OF rels_lemma])
+  apply(subst Let_def)
+  apply(simp only: the_elem_lemma)
+  apply(subst Let_def)
+  apply(simp only: word_calc_lemma)
 
 theorem at_least_some_relocations_relocate:
     fixes ef :: elf64_file and segs_and_provenance :: "(elf64_interpreted_segment \<times> segment_provenance) list" and entry :: "nat"
             and rstate final_fixed_state final_relocatable_state :: "X64_state"
-  assumes "ef = elf64_file_of_elf_memory_image sysv_amd64_std_abi id ''at_least_some_relocations_relocate.out'' relocation_image"
-      and "Success (segs_and_provenance, entry, elf_ma_x86_64) = get_elf64_executable_image ef"
-      and "rstate = load_image (List.map fst segs_and_provenance) entry"
-      and "final_fixed_state = run_program fixed_program initial_state"
+  assumes "i = elements relocation_image" and "entry = 4194304"
+      and "rstate = load_image i entry"
+      and "final_fixed_state = run_program fixed_program (initial_state entry)"
       and "final_relocatable_state = execute_two_steps rstate"
     shows "REG final_fixed_state = REG final_relocatable_state" (* XXX: probably want to say something about the contents of memory here, too! *)
-using assms(1)
-  apply(simp only: elf64_file_of_elf_memory_image_def)
-  apply(simp only: elf_memory_image_section_ranges_def)
-  apply(simp only: tagged_ranges_matching_tag_def)
+using assms
   apply(simp only: relocation_image_def)
   apply(simp only: relocatable_program_def)
-  apply(simp only: if_True)
-  apply(simp only: silly_map_lemma1)
+  apply(simp only: List.list.map)
+  apply(simp only: mov_constant_to_mem_def mov_constant_from_mem_def)
+  apply(simp only: encode.simps)
+  apply(simp only: X64.instruction.case split X64.Zcond.case Zsize.case Zdest_src.case Zrm.case)
+  apply(simp only: List.concat.simps)
   apply(simp only: img1_def)
-  apply(simp only: silly_map_lemma2)
-  apply(simp only: silly_rev_lemma1)
-  apply(simp only: silly_map_of_lemma1)
-  apply(simp only: silly_rev_lemma2)
-  apply(simp only: silly_map_of_lemma2)
+  apply(simp only: rev.simps append.simps map_of.simps fst_def snd_def split)
+  apply(simp only: Let_def append_Nil2)
+  apply(simp only: meta0_def set_simps by_tag_from_by_range_def swap_pairs_lemma)
+  apply(simp only: map_append)
+  apply(simp only: relocate_output_image_def)
+  apply(simp only: annotated_memory_image.simps)
+  apply(simp only: lookupBy0_def)
+  apply(case_tac "findLowestKVWithKEquivTo (instance_Basic_classes_Ord_Memory_image_range_tag_dict instance_Basic_classes_Ord_Abis_any_abi_feature_dict)
+                          (instance_Basic_classes_Ord_Maybe_maybe_dict
+                            (instance_Basic_classes_Ord_tup2_dict instance_Basic_classes_Ord_string_dict
+                              (instance_Basic_classes_Ord_tup2_dict instance_Basic_classes_Ord_Num_natural_dict instance_Basic_classes_Ord_Num_natural_dict)))
+                          (SymbolRef null_symbol_reference_and_reloc_site) (tagEquiv instance_Abi_classes_AbiFeatureTagEquiv_Abis_any_abi_feature_dict)
+                          {(SymbolRef ref_and_reloc_rec0, Some (''.text'', 1\<Colon>nat, 4\<Colon>nat)), (SymbolDef def_rec0, Some (''.data'', 0\<Colon>nat, 8\<Colon>nat))} None")
+  apply(simp only: Let_def)
+  apply(simp only: option.case foldl.simps annotated_memory_image.simps)
+  apply(simp only: execute_two_steps_def load_image_def)
+  apply(simp only: Let_def)
+
 
 end
